EpsilonNFA as special case of NFA

AutoKchp/NatEpsNFA.lean
@@ -6,30 +6,59 @@ Authors: Marc Perlade
 
 module
 
+public import AutoKchp.NFA
+
 @[expose]
 public section
 
-structure NatEpsNFA (a: Nat) where
-  n: Nat
-  δ: Fin n → Option (Fin a) → (Array (Fin n))
-  i: Array (Fin n)
-  f: Fin n → Bool
+def NatEpsNFA (a: Nat) := NatNFA (a + 1)
 
 namespace NatEpsNFA
 
-inductive path {a: Nat} (r: NatEpsNFA a): Fin r.n → Fin r.n → List (Fin a) → Prop where
-  | refl (p: Fin r.n): r.path p p []
-  | trans {b: Fin a} {t: List (Fin a)} {p q u: Fin r.n}:
-    u ∈ r.δ p (some b) → r.path u q t → r.path p q (b::t)
-  | eps {l: List (Fin a)} {p q u: Fin r.n}:
-    u ∈ r.δ p none → r.path u q l → r.path p q l
+def ε {a: Nat}: Fin (a + 1) := ⟨a, Nat.lt_succ_self a⟩
+
+
+def char {a: Nat} (c: Fin a): Fin (a + 1) := ⟨c.val, Nat.lt_succ_of_lt c.isLt⟩
+
+
+def extractWord {a: Nat}: List (Fin (a + 1)) → List (Fin a)
+  | [] => []
+  | b::t => if eq: b = ε
+    then extractWord t
+    else ⟨b.val, Nat.lt_of_le_of_ne (Nat.le_of_lt_succ b.isLt)
+      (Fin.val_ne_of_ne eq)⟩::(extractWord t)
+
+
+theorem extractWord_cons_ε {a: Nat} {l: List (Fin (a + 1))}:
+    extractWord (ε::l) = extractWord l :=
+  dif_pos rfl
+
+
+theorem extractWord_cons_char {a: Nat} {l: List (Fin (a + 1))} {b: Fin a}:
+    extractWord ((char b)::l) = b::(extractWord l) :=
+  dif_neg (Fin.ne_of_val_ne (Nat.ne_of_lt b.isLt))
+
+
+theorem extractWord_append {a: Nat} {f g: List (Fin (a + 1))}:
+    extractWord (f ++ g) = extractWord f ++ extractWord g :=
+  match f with
+  | [] => rfl
+  | b::t => if eq: b = ε then
+      (dif_pos eq).trans ((extractWord_append (f := t) (g := g)).trans
+        (congrArg (· ++ extractWord g) (dif_pos eq (t := fun _ => extractWord t)).symm))
+    else
+      (dif_neg eq).trans ((List.cons_eq_cons.mpr ⟨rfl, extractWord_append⟩).trans
+        (congrArg (· ++ extractWord g) (dif_neg eq (e := fun _ => _::(extractWord t))).symm))
+
+
+def path {a: Nat} (r: NatEpsNFA a): Fin r.n → Fin r.n → List (Fin a) → Prop :=
+  fun p q l => ∃ u: List (Fin (a + 1)), l = extractWord u ∧ (NatNFA.path r p q u)
 
 
 theorem join_paths {a: Nat} {r: NatEpsNFA a} {i j k: Fin r.n} {u v: List (Fin a)}:
-    r.path i j u → r.path j k v → r.path i k (u ++ v)
-  | path.refl i => id
-  | path.trans h1 h2 => fun h3 => path.trans h1 (join_paths h2 h3)
-  | path.eps h1 h2 => fun h3 => path.eps h1 (join_paths h2 h3)
+    r.path i j u → r.path j k v → r.path i k (u ++ v) :=
+  fun ⟨f, eqf, hf⟩ ⟨g, eqg, hg⟩ =>
+    ⟨f ++ g, eqf ▸ eqg ▸ extractWord_append.symm, NatNFA.join_paths hf hg⟩
 
 
 def successfulPath {a: Nat} (r: NatEpsNFA a) (p q: Fin r.n) (l: List (Fin a)): Prop :=
